LL1/Proofs/ParseTableGen/EndToEnd.v
@@ -4,20 +4,20 @@ Require Import LL1.ParseTable.
 Require Import LL1.Proofs.ParseTableGen.tableFromEntries_Correctness.
 Require Import LL1.Proofs.ParseTableGen.tableEntries_Correctness.
 
-Theorem mkParseTable_sound : 
+Theorem genTableForGrammar_sound : 
   forall g nu fi fo tbl,
   nullable_set_for nu g
   -> first_map_for fi g
   -> follow_map_for fo g
-  -> mkParseTable g nu fi fo = Some tbl
+  -> genTableForGrammar g nu fi fo = Some tbl
   -> parse_table_for tbl g.
 Proof.
   intros g nu fi fo tbl Hnu Hfi Hfo Hmk.
-  eapply tableFromEntries_sound; eauto.
-  eapply tableEntries_correct; eauto.
+  eapply mkParseTable_sound; eauto.
+  eapply mkEntries_correct; eauto.
 Qed.
 
-Theorem mkParseTable_complete :
+Theorem genTableForGrammar_complete :
   forall g nu fi fo tbl,
     nullable_set_for nu g
     -> first_map_for fi g
@@ -25,9 +25,10 @@ Theorem mkParseTable_complete :
     -> parse_table_for tbl g
     -> exists tbl',
         ParseTable.Equal tbl tbl'
-        /\ mkParseTable g nu fi fo = Some tbl'.
+        /\ genTableForGrammar g nu fi fo = Some tbl'.
 Proof.
   intros g nu fi fo tbl Hnu Hfi Hfo Hpt.
-  eapply tableFromEntries_complete; eauto.
-  eapply tableEntries_correct; eauto.
+  eapply mkParseTable_complete; eauto.
+  eapply mkEntries_correct; eauto.
 Qed.
+
